WIP on vectors.

src/vector.v
@@ -15,32 +15,59 @@ Open Scope nat_scope.
 
 (* A vector is a pair of a logical length [_n] and an array [a]. *)
 
-Definition vectorInv `{Inhabited A} _n a (xs : list A) :=
-  ∃ unoccupied,
-  isInt _n (len xs) ∧
-  isArray a (xs ++ unoccupied).
-
 Definition vector (A : Type) :=
   (int * array A)%type.
 
-Definition isVector `{Inhabited A} (v : vector A) (xs : list A) :=
-  let (_n, a) := v in
-  vectorInv _n a xs.
+(* The proposition [isVectorCap v xs c] means that [v] is a vector whose
+   logical content is [xs] and whose capacity is [c]. *)
 
-(* These tactics and lemmas help work with [isVector]. *)
+Definition isVectorCap `{Inhabited A} (v : vector A) (xs : list A) c :=
+  let (_n, a) := v in
+  ∃ unoccupied,
+  isInt _n (len xs) ∧
+  isArray a (xs ++ unoccupied) ∧
+  len xs + len unoccupied = c.
+
+(* The proposition [isVector v xs] means that [v] is a vector whose
+   logical content is [xs]. *)
+
+Definition isVector `{Inhabited A} (v : vector A) (xs : list A) :=
+  ∃ c, isVectorCap v xs c.
+
+(* These tactics and lemmas help work with the above propositions. *)
 
 Local Ltac introIsVector :=
-  unfold isVector; unfold vectorInv; eexists; list; split.
+  unfold isVector; eexists.
 
-Local Ltac introIsVectorWithWitness u :=
-  unfold isVector; unfold vectorInv; exists u; list; split.
+Local Ltac introIsVectorCap :=
+  unfold isVectorCap; eexists; list;
+  split; [| split ].
 
-Local Ltac destructIsVector _n a :=
+Local Ltac introIsVectorCapWithWitness unoccupied :=
+  unfold isVectorCap; exists unoccupied; list;
+  split; [| split ].
+
+Local Ltac destructIsVector :=
   match goal with h: isVector ?v _ |- _ =>
-    destruct v as [ _n a ];
     unfold isVector in h;
+    let c := fresh "c" in
+    destruct h as (c&?)
+  end.
+
+Local Ltac destructVector v :=
+  match v with
+  | (_, _) => idtac
+  | _ =>
+    let _n := fresh "_n" in
+    let a := fresh "a" in
+    destruct v as [ _n a ]
+  end.
+
+Local Ltac destructIsVectorCap :=
+  match goal with h: isVectorCap ?v _ _ |- _ =>
+    destructVector v;
     let u := fresh "unoccupied" in
-    destruct h as (u&?&?)
+    destruct h as (u&?&?&?)
   end.
 
 (* -------------------------------------------------------------------------- *)
@@ -49,6 +76,7 @@ Section Operations.
 Context `{Inhabited A}.
 Implicit Types v : vector A.
 Implicit Types xs : list A.
+Implicit Types a b : array A.
 
 (* -------------------------------------------------------------------------- *)
 
@@ -64,7 +92,8 @@ Definition create (_ : unit) : vector A :=
 Lemma wp_create :
   wp (create ()) (λ v, isVector v []).
 Proof.
-  unfold create. wp_make a. wp_ret. introIsVector; eauto with int.
+  unfold create. wp_make a. wp_ret.
+  introIsVector. introIsVectorCap; eauto with int.
 Qed.
 
 (* -------------------------------------------------------------------------- *)
@@ -81,7 +110,9 @@ Lemma wp_get v xs _i i :
   valid i xs →
   wp (get v _i) (λ x, x = xs !!! i).
 Proof.
-  intros. unfold get. destructIsVector _n a. wp_get x. eauto.
+  intros. unfold get.
+  destructIsVector. destructIsVectorCap.
+  wp_get x. eauto.
 Qed.
 
 Definition set v _i x : vector A :=
@@ -95,8 +126,10 @@ Lemma wp_set v xs _i i x :
   valid i xs →
   wp (set v _i x) (λ v', isVector v' (<[i := x]>xs)).
 Proof.
-  intros. unfold set. destructIsVector _n a.
-  wp_set. wp_ret. introIsVector; eauto.
+  intros. unfold set.
+  destructIsVector. destructIsVectorCap.
+  wp_set. wp_ret.
+  introIsVector. introIsVectorCap; eauto.
 Qed.
 
 (* -------------------------------------------------------------------------- *)
@@ -120,17 +153,122 @@ Lemma wp_pop v xs :
     isVector v (initial_seg i xs)
   ).
 Proof.
-  intros. unfold pop. destructIsVector _n a.
+  intros. unfold pop.
+  destructIsVector. destructIsVectorCap.
   wp_get x. wp_ret. split; [ eauto |].
-  introIsVectorWithWitness ({[x]} ++ unoccupied).
-  + eauto with int.
-  + subst x. isArray.
+  introIsVector.
+  introIsVectorCapWithWitness ({[x]} ++ unoccupied); eauto with int.
+  subst x. isArray.
 Qed.
 
 (* -------------------------------------------------------------------------- *)
 
+(* Growing a vector requires allocating a new array and migrating
+   the existing data into it. *)
+
+(* In [grow v _c], [_c] is the desired capacity of the new array. *)
+
+(* [grow] is an internal function. It returns just the new array,
+   not a vector. The logical length of the vector is unchanged. *)
+
+Local Definition grow v _c : array A :=
+  let '(_n, a) := v in
+  do b ← make _c inhabitant ;
+  do b ← blit a 0 b 0 _n ;
+  b.
+
+Local Lemma wp_grow _n a xs _c c :
+  isVector (_n, a) xs →
+  isInt _c c →
+  len xs ≤ c ≤ max_array_length →
+  wp (grow (_n, a) _c) (λ b,
+    isVectorCap (_n, b) xs c
+  ).
+Proof.
+  intros. unfold grow.
+  destructIsVector. destructIsVectorCap.
+  wp_make b. wp_blit. wp_ret.
+  introIsVectorCap; eauto with int.
+  list. lia.
+Qed.
+
+(* -------------------------------------------------------------------------- *)
+
+(* TODO WIP here *)
+
+Definition capacity v : int :=
+  let '(_, a) := v in
+  length a.
+
+Local Definition next_capacity _c : int :=
+  do _k ← (
+    if (_c ≤? 512)%uint63 then (_c * 2)%uint63
+    else (_c + _c / 2)%uint63
+  ) ;
+  _min max_length (_max 8%uint63 _k).
+
+(* TODO *
+Hint Extern 1 (isInt _ _) =>
+  match goal with
+  | |- isInt ?_i ?i =>
+    is_evar _i
+  | |- isInt ?_i ?i =>
+    eapply introIsInt'
+  end;
+  fail "evar"
+: int.
+ *)
+
+Lemma isInt_next_capacity _c c :
+  isInt _c c →
+  c ≤ max_array_length →
+  wp (next_capacity _c) (λ _c', ∃ c',
+    isInt _c' c' ∧ c ≤ c' ∧ c' ≤ max_array_length
+  ).
+Proof.
+  intros. unfold next_capacity.
+  eapply wp_bind with (P := λ _c', ∃ c',
+    isInt _c' c' ∧ c ≤ c' ∧ representable c').
+  {
+    (* Lots of preliminary remarks about machine integers. *)
+    assert (isInt 2 2) by eauto with int. (* TODO *)
+    assert (isInt 512 512) by eauto with int. (* TODO *)
+
+    generalize representable_twice_max_array_length; intro.
+    assert (representable (c * 2)).
+    { rewrite representable_iff_nat in *. lia. }
+    assert (representable (c + c `div` 2)).
+    { assert (c `div` 2 ≤ c) by eauto with lia.
+      rewrite representable_iff_nat in *. lia. }
+    (* Now conclude. *)
+     wp_if; wp_ret; eauto 7 with int lia representable.
+  }
+  intros _k (c'&?&?&?).
+  wp_ret.
+  (* Another remark. *)
+  assert (isInt 8 8) by eauto with int. (* TODO *)
+  (* (* Now conclude. *) *)
+  (* This proof is not as concise as I would like.
+     [eauto] with hints does not work as expected. *)
+  eexists. split.
+  { eapply isInt_min.
+    + eauto using max_length_spec.
+    + eauto with int representable.
+    + eauto with representable.
+    + eauto using max_representable with representable. }
+  { lia. }
+Qed.
+
 (* TODO *)
-Variable really_ensure_capacity : vector A → int → array A.
+(* _r : request *)
+(* _c : capacity *)
+Definition really_ensure_capacity v _r : array A :=
+  do _c ← capacity v ;
+  do _c' ← (
+    if (_r ≤? _c)%uint63 then _c
+    else _max (next_capacity _c) _r
+  ) ;
+  grow v _c'.
 
 Lemma wp_really_ensure_capacity v xs _n' n' :
   isInt _n' n' →
@@ -152,9 +290,9 @@ Definition push v x : vector A :=
   let (_n, a) := v in
   (* Ensure that sufficient space exists. *)
   let _n' := (_n + 1)%uint63 in
-  do capacity ← length a ;
+  do _c ← length a ;
   do a ← (
-    if (_n' ≤? capacity)%uint63 then a
+    if (_n' ≤? _c)%uint63 then a
     else really_ensure_capacity v _n'
   ) ;
   (* A free slot now exists. *)
@@ -166,8 +304,9 @@ Lemma wp_push v xs x :
   len xs + 1 ≤ max_array_length →
   wp (push v x) (λ v, isVector v (xs ++ {[x]})).
 Proof.
-  intros. cbv delta [ push ]. destructIsVector _n a.
-  wp_length capacity.
+  intros. unfold push.
+  destructIsVector. destructIsVectorCap.
+  wp_length _c.
   (* We are looking at the [if] construct. At the join point,
      at least one free slot exists in the array. *)
   eapply wp_bind with (P := λ a,
@@ -184,10 +323,10 @@ Proof.
   clear dependent a unoccupied. intros a (unoccupied & ? & ?).
   (* Write; return. *)
   wp_set. wp_ret.
-  introIsVectorWithWitness (final_seg 1 unoccupied).
-  + eauto with int.
-  + isArray.
-    rewrite (seg_intro unoccupied) at 1. list. eauto.
+  introIsVector.
+  introIsVectorCapWithWitness (final_seg 1 unoccupied); eauto with int.
+  isArray.
+  rewrite (seg_intro unoccupied) at 1. list. eauto.
 Qed.
 
 (* -------------------------------------------------------------------------- *)
